VNM.v
@@ -5,7 +5,7 @@ Require Extraction.
 Extraction Language Haskell.
 
 Parameter assignment : Observable -> Player -> nat.
-Parameter o0 : Observable.
+
 Definition reachable_payoffs_property (g:CGS)
          (q:State)
          (c:coalition)
@@ -13,55 +13,44 @@ Definition reachable_payoffs_property (g:CGS)
   : Prop :=
   forall (p:Player),
     c p ->
-    @verifies g q (<< c >>^ (obs o)).
+    verifies g q (<< c >>^ (obs o)).
 
 Check reachable_payoffs_property.
-
-Definition reachable_payoffs (g:CGS) (q:State) (c:coalition) : Set
-           := {o:Observable | reachable_payoffs_property g q c o}.
 
 Definition spec_reachable_payoffs_property (sp:spec)
            (q:State)
            (c:coalition)
            (o:Observable)
   :=
-    forall (phi:sentence) (g:CGS), sp phi ->
-                                   @verifies g q phi ->
-                                   reachable_payoffs_property g q c o.
+    forall(g:CGS), g_in_spec sp g q ->
+                             reachable_payoffs_property g q c o.
 
 Definition spec_reachable_payoffs (sp:spec) (q:State) (c:coalition) : Type
   := {o:Observable | spec_reachable_payoffs_property sp q c o}.
 
-Definition core (g:CGS) (q:State) (c:coalition) (o: Observable)  : Prop :=
-  @verifies g q ( <<c>>^ obs o )
-  /\ forall (p:Player) (r:reachable_payoffs g q c) (c':coalition),
-    let o' := proj1_sig r in
-    c p -> c' p -> assignment o' p < assignment o p.
+Definition core (g:CGS) (q:State) (o: Observable)  : Prop :=
+  exists c:coalition,
+    reachable_payoffs_property g q c o
+    /\ (forall (o':Observable), (* Efficiency *)
+            reachable_payoffs_property g q c o' ->
+            (forall (p:Player),
+              assignment o' p <= assignment o p))
+    /\ (forall (o':Observable),
+           ~(exists (c':coalition),
+                reachable_payoffs_property g q c' o' /\
+                (forall (p:Player),
+                    c p ->
+                    c' p ->
+                    assignment o' p <= assignment o p))).
 
 Definition listp_to_coalition (lp:list Player) : coalition := fun p => In p lp.
 
-Definition core' (g:CGS) (q:State) (lo:list Observable): list  (Observable * (list coalition))
-  :=let c_helper
-        := fix ch (current: list Player) (o:Observable)
-             := match current with
-                | nil => true
-                | p::current' => 
-                  if
-                    fold_left (fun b o' =>
-                                 andb b (leb (assignment o' p)
-                                             (assignment o p)))
-                              lo true
-                  then ch current' o
-                  else false
-                end
-    in
-    let helper
-        := fix fh (remaining current :list Player) (result:list (list Player)) (o:Observable)
-             := match remaining with
-                | nil => if c_helper current o then current::result else result
-                | p::remaining' =>
-                   let r := fh remaining' (p::current) result o
-                   in fh remaining' current r o
-                end
-    in (map (fun o => (o, (map listp_to_coalition (helper g.(lp) nil nil o))))
-                      lo).
+Axiom core_must_happen : forall (g:CGS) (q:State) (o:Observable),
+    core g q o -> reachable_payoffs_property g q (fun _:Player => False) o.
+
+Theorem sp_core_must_happen : forall (sp:spec) (o:Observable) (c:coalition) (g:CGS) (q:State),
+    g_in_spec sp g q -> core g q o -> reachable_payoffs_property g q (fun _:Player => False) o.
+Proof.
+  intros. apply core_must_happen. apply H0.
+Qed.
+
